#+TITLE:
#+AUTHOR:
#+LANGUAGE:  en
#+OPTIONS:   H:3 num:t toc:nil \n:nil @:t ::t |:t ^:t -:t f:t *:t <:t
#+OPTIONS:   TeX:t LaTeX:t skip:nil d:nil todo:t pri:nil tags:not-in-toc
#+INFOJS_OPT: view:nil toc:nil ltoc:t mouse:underline buttons:0 path:http://orgmode.org/org-info.js
#+EXPORT_SELECT_TAGS: export
#+EXPORT_EXCLUDE_TAGS: noexport
#+LINK_UP:
#+LINK_HOME:
#+XSLT:
#+LaTeX_HEADER: \usepackage{amsmath, amsthm, amssymb, breqn}
#+LaTeX_HEADER: \usepackage[margin=1in]{geometry}

\noindent{}KEITH DEVLIN: Introduction to Mathematical Thinking (Fall 2013)\hfill Final Exam \\
\\ \\
\centerline{\underline{QUESTION 3}} \\
\\ \\
\textbf{Theorem} for any integer \(n\), \(n^2 + n + 1\) is odd. \\
\\
\emph{Proof:} by consideration of even/odd cases. \\
\\
(i) Assume \(n\) is even. Then \(n = 2k\).
\begin{align*}
n^2 + n + 1 & = (2k)^2 + 2k + 1 \\
& = 4k^2 + 2k + 1 \\
& = 2(2k^2 + k) + 1
\end{align*}
Therefore, \(n\) is even \(\Rightarrow n^2 + n + 1\) is odd. \\
\\
(ii) Assume \(n\) is odd. Then \(n = 2k + 1\).
\begin{align*}
n^2 + n + 1 & = (2k + 1)^2 + (2k + 1) + 1 \\
& = 4k^2 + 4k + 1 + 2k + 1 + 1 \\
& = 4k^2 + 6k + 2 + 1 \\
& = 2(2k^2 + 3k + 1) + 1
\end{align*}
Therefore, \(n\) is odd \(\Rightarrow n^2 + n + 1\) is odd. \\
\\
Therefore for any integer \(n\), \(n^2 + n + 1\) is odd.\qed
