#+TITLE:
#+AUTHOR:
#+LANGUAGE:  en
#+OPTIONS:   H:3 num:t toc:nil \n:nil @:t ::t |:t ^:t -:t f:t *:t <:t
#+OPTIONS:   TeX:t LaTeX:t skip:nil d:nil todo:t pri:nil tags:not-in-toc
#+INFOJS_OPT: view:nil toc:nil ltoc:t mouse:underline buttons:0 path:http://orgmode.org/org-info.js
#+EXPORT_SELECT_TAGS: export
#+EXPORT_EXCLUDE_TAGS: noexport
#+LINK_UP:
#+LINK_HOME:
#+XSLT:
#+LaTeX_HEADER: \usepackage{amsmath, amsthm, amssymb, breqn}
#+LaTeX_HEADER: \usepackage[margin=1in]{geometry}

\noindent{}KEITH DEVLIN: Introduction to Mathematical Thinking (Fall 2013)\hfill Final Exam \\
\\ \\
\centerline{\underline{QUESTION 4}} \\
\\ \\
\textbf{Theorem} every odd natural number is one of the forms \(4n + 1\) or \(4n + 3\) where \(n\in\mathbb{Z}\). \\
\\
\emph{Proof:} by induction, considering each case. \\
\\
Base case: \(1 = 4n + 1\) where \(n = 0\). \\
\\
Inductive step: If \(k_i\) is an odd natural number, the next odd natural number is given by \(k_{i+1} = k_i + 2\). \\
There are two cases to consider. \\
\\
(i) Assume \(k_i = 4n + 1\). Then:
\begin{align*}
k_{i+1} & = k_i + 2 \\
& = 4n + 1 + 2 \tag{by induction hypothesis}\\
& = 4n + 3
\end{align*}
Therefore, \(k_{i+1}\) is of the required form.\\
\\
(ii) Assume \(k_i = 4n + 3\). Then:
\begin{align*}
k_{i+1} & = k_i + 2 \\
& = 4n + 3 + 2 \tag{by induction hypothesis}\\
& = 4n + 4 + 1 \\
& = 4(n+1) + 1
\end{align*}
Therefore, \(k_{i+1}\) is again of the required form.\\
\\
Therefore every odd natural number is one of the forms \(4n + 1\) or \(4n + 3\) where \(n\in\mathbb{Z}\).\qed
