#+TITLE:
#+AUTHOR:
#+LANGUAGE:  en
#+OPTIONS:   H:3 num:t toc:nil \n:nil @:t ::t |:t ^:t -:t f:t *:t <:t
#+OPTIONS:   TeX:t LaTeX:t skip:nil d:nil todo:t pri:nil tags:not-in-toc
#+INFOJS_OPT: view:nil toc:nil ltoc:t mouse:underline buttons:0 path:http://orgmode.org/org-info.js
#+EXPORT_SELECT_TAGS: export
#+EXPORT_EXCLUDE_TAGS: noexport
#+LINK_UP:
#+LINK_HOME:
#+XSLT:
#+LaTeX_HEADER: \usepackage{amsmath, amsthm, amssymb, breqn}
#+LaTeX_HEADER: \usepackage[margin=1in]{geometry}

\noindent{}KEITH DEVLIN: Introduction to Mathematical Thinking (Fall 2013)\hfill Final Exam \\
\\ \\
\centerline{\underline{QUESTION 7}} \\
\\ \\
\textbf{Theorem} \((\forall{}n\in\mathbb{N})(2 + 2^2 + 2^3 + ... + 2^n = 2^{n+1} - 2)\)\\
\\
\emph{Proof:} by induction.\\
\\
Base case: When \(n = 1\), \(2^n = 2^1 = 2 = 2^2 - 2\). \\
\\
Inductive step: Assume the identity holds for \(n\). Then:
\begin{align*}
2 + 2^2 + 2^3 + ... + 2^{n+1} & = 2 + 2^2 + 2^3 + ... + 2^n + 2^{n+1}\\
& = 2^{n+1} - 2 + 2^{n+1}\tag{by induction hypothesis}\\
& = 2(2^{n+1}) - 2\\
& = 2^{n+2} - 2
\end{align*}
which establishes the identity for \(n+1\).\\
\\
Therefore \((\forall{}n\in\mathbb{N})(2 + 2^2 + 2^3 + ... + 2^n = 2^{n+1} - 2)\).\qed
